schedule.md
@@ -5,14 +5,18 @@ permalink: /schedule/
 ---
 
 | # | Topic | Dates | Materials | Comments | 
-|--:|-------|-------|-----------|----------|
-| 1 | First day of class | 16/01 | slides ([pdf](https://kcsrk.info/cs6225_s25_iitm/lectures/0_first_day_of_classes.pdf), [key](https://kcsrk.info/cs6225_s21_iitm/lectures/0_first_day_of_classes.pdf)) | [Benjamin Pierce, "Lambda the Ultimate TA"](https://vimeo.com/6615365), <br/> [Terence Tao, "AI and Mathematics"](https://www.youtube.com/watch?v=e049IoFBnLA), <br/> [Terence Tao, "Machine assisted Proofs"](https://www.ams.org/journals/notices/202501/rnoti-p6.pdf) |
-| 2 | Functional Programming | 17/01, 20/01 | [Coq](https://github.com/kayceesrk/cs6225_s25_iitm/blob/main/lectures/FunctionalProgramming.v) | |
-| 3 | Logic | 20/01, 22/01, 23/01 | [Coq](https://github.com/kayceesrk/cs6225_s25_iitm/blob/main/lectures/Logic.v) | |
-| 4 | Induction | 23/01, 24/01, 27/01 | [Coq](https://github.com/kayceesrk/cs6225_s25_iitm/blob/main/lectures/Induction.v) | |
-| 5 | BasicSyntax | 29/01, 30/01, 31/01 | [Coq](https://github.com/kayceesrk/cs6225_s25_iitm/blob/main/lectures/BasicSyntax.v) | |
-| 6 | Interpreters | 31/01, 03/02, 06/02 | [Coq](https://github.com/kayceesrk/cs6225_s25_iitm/blob/main/lectures/Interpreters.v),  [slides (key)]({{site.baseurl}}/lectures/1_interpreters.key), [slides (pdf)]({{site.baseurl}}/lectures/1_interpreters.pdf) | |
-| 7 | Logic Programming | 07/02, 12/02 | [Coq](https://github.com/kayceesrk/cs6225_s25_iitm/blob/main/lectures/LogicProgramming.v) | c.f. CS3100 Prolog parts |
-| 7 | Functional Programming in F\* | 13/02, 14/02 | [slides(key)]({{site.baseurl}}/lectures/2_fstar_functional_programming.key), [slides(pdf)]({{site.baseurl}}/lectures/2_fstar_functional_programming.pdf), [fst]({{site.baseurl}}/lectures/Fstar_functional.fst) | See F* book mentioned in [resources]({{site.baseurl}}/resources/) |
-| 8 | Verifying Functional Programs in F\* | | [fst]({{site.baseurl}}/lectures/Fstar_verification.fst) | |
-
+|---:|-------|-------|-----------|----------|
+|  1 | First day of class | 16/01 | slides ([pdf](https://kcsrk.info/cs6225_s25_iitm/lectures/0_first_day_of_classes.pdf), [key](https://kcsrk.info/cs6225_s21_iitm/lectures/0_first_day_of_classes.pdf)) | [Benjamin Pierce, "Lambda the Ultimate TA"](https://vimeo.com/6615365), <br/> [Terence Tao, "AI and Mathematics"](https://www.youtube.com/watch?v=e049IoFBnLA), <br/> [Terence Tao, "Machine assisted Proofs"](https://www.ams.org/journals/notices/202501/rnoti-p6.pdf) |
+|  2 | Functional Programming | 17/01, 20/01 | [Coq](https://github.com/kayceesrk/cs6225_s25_iitm/blob/main/lectures/FunctionalProgramming.v) | |
+|  3 | Logic | 20/01, 22/01, 23/01 | [Coq](https://github.com/kayceesrk/cs6225_s25_iitm/blob/main/lectures/Logic.v) | |
+|  4 | Induction | 23/01, 24/01, 27/01 | [Coq](https://github.com/kayceesrk/cs6225_s25_iitm/blob/main/lectures/Induction.v) | |
+|  5 | BasicSyntax | 29/01, 30/01, 31/01 | [Coq](https://github.com/kayceesrk/cs6225_s25_iitm/blob/main/lectures/BasicSyntax.v) | |
+|  6 | Interpreters | 31/01, 03/02, 06/02 | [Coq](https://github.com/kayceesrk/cs6225_s25_iitm/blob/main/lectures/Interpreters.v),  [slides (key)]({{site.baseurl}}/lectures/1_interpreters.key), [slides (pdf)]({{site.baseurl}}/lectures/1_interpreters.pdf) | |
+|  7 | Logic Programming | 07/02, 12/02 | [Coq](https://github.com/kayceesrk/cs6225_s25_iitm/blob/main/lectures/LogicProgramming.v) | c.f. CS3100 Prolog parts |
+|  8 | Functional Programming in F\* | 13/02, 14/02 | [slides(key)]({{site.baseurl}}/lectures/2_fstar_functional_programming.key), [slides(pdf)]({{site.baseurl}}/lectures/2_fstar_functional_programming.pdf), [fst]({{site.baseurl}}/lectures/Fstar_functional.fst) | See F* book mentioned in [resources]({{site.baseurl}}/resources/) |
+|  9 | Verifying Functional Programs in F\* | | [fst]({{site.baseurl}}/lectures/Fstar_verification.fst) | |
+| 10 | Transition Systems | | | |
+| 11 | Operational Semantics | | | |
+| 12 | Lambda Calculus | | | |
+| 13 | Hoare Logic | | | | 
+| 14 | Effectful Programming in F\* | | | |
